raw_equiv_list_no_map

src/cbor/CBOR.Spec.Raw.fsti
@@ -457,75 +457,217 @@ let raw_data_item_sorted_optimal_valid
     )
     x1
 
-let map_key_not_map
-  (x: (raw_data_item & raw_data_item))
-: Tot bool
-= not (Map? (fst x))
+val raw_data_item_size
+  (x: raw_data_item)
+: Tot nat
 
-let no_map_and_no_repeats_keys_map
-  (v: list (raw_data_item & raw_data_item))
-: Tot bool
-= List.Tot.for_all map_key_not_map v &&
-  List.Tot.noRepeats (List.Tot.map fst v)
+val raw_data_item_size_eq
+  (x: raw_data_item)
+: Lemma
+  (raw_data_item_size x == begin match x with
+  | Array _ v -> 2 + list_sum raw_data_item_size v
+  | Map _ v -> 2 + list_sum (pair_sum raw_data_item_size raw_data_item_size) v
+  | Tagged _ v -> 2 + raw_data_item_size v
+  | _ -> 1
+  end)
 
-let no_map_and_no_repeats_keys_elem
+let rec raw_equiv_list_no_map
+  (l1 l2: list raw_data_item)
+: Tot bool
+  (decreases (list_sum raw_data_item_size l1))
+= match l1, l2 with
+  | [], [] -> true
+  | x1 :: q1, x2 :: q2 ->
+    raw_data_item_size_eq x1;
+    begin match x1, x2 with
+    | Simple v1, Simple v2 -> v1 = v2 && raw_equiv_list_no_map q1 q2
+    | Int64 ty1 v1, Int64 ty2 v2 -> ty1 = ty2 && raw_uint64_equiv v1 v2 && raw_equiv_list_no_map q1 q2
+    | String ty1 len1 v1, String ty2 len2 v2 -> ty1 = ty2 && raw_uint64_equiv len1 len2 && v1 = v2 && raw_equiv_list_no_map q1 q2
+    | Array len1 v1, Array len2 v2 ->
+      list_sum_append raw_data_item_size v1 q1;
+      raw_uint64_equiv len1 len2 &&
+      raw_equiv_list_no_map (List.Tot.append v1 q1) (List.Tot.append v2 q2)
+    | Tagged tag1 v1, Tagged tag2 v2 ->
+      raw_uint64_equiv tag1 tag2 &&
+      raw_equiv_list_no_map (v1 :: q1) (v2 :: q2)
+    | _ -> false
+    end
+  | _ -> false
+
+let rec raw_equiv_list_no_map_append
+  (ll1 lr1 ll2 lr2: list raw_data_item)
+: Lemma
+  (requires (List.Tot.length ll1 == List.Tot.length ll2))
+  (ensures (raw_equiv_list_no_map (List.Tot.append ll1 lr1) (List.Tot.append ll2 lr2) == (raw_equiv_list_no_map ll1 ll2 && raw_equiv_list_no_map lr1 lr2)))
+  (decreases (list_sum raw_data_item_size ll1))
+= match ll1, ll2 with
+  | x1 :: q1, x2 :: q2 ->
+    raw_data_item_size_eq x1;
+    begin match x1, x2 with
+    | Tagged tag1 v1, Tagged tag2 v2 ->
+      raw_equiv_list_no_map_append (v1 :: q1) lr1 (v2 :: q2) lr2
+    | Array len1 v1, Array len2 v2 ->
+      list_sum_append raw_data_item_size v1 q1;
+      if raw_uint64_equiv len1 len2
+      then begin
+        assert (List.Tot.length v1 == List.Tot.length v2);
+        List.Tot.append_assoc v1 q1 lr1;
+        List.Tot.append_assoc v2 q2 lr2;
+        List.Tot.append_length v1 q1;
+        List.Tot.append_length v2 q2;
+        raw_equiv_list_no_map_append (List.Tot.append v1 q1) lr1 (List.Tot.append v2 q2) lr2
+      end
+    | _ -> raw_equiv_list_no_map_append q1 lr1 q2 lr2
+    end
+  | _ -> ()
+
+let rec raw_equiv_list_no_map_no_map
+  (l1 l2: list raw_data_item)
+: Lemma
+  (requires (raw_equiv_list_no_map l1 l2 == true))
+  (ensures (List.Tot.for_all (holds_on_raw_data_item (notp Map?)) l1 == true))
+  (decreases (list_sum raw_data_item_size l1))
+= match l1, l2 with
+  | x1 :: q1, x2 :: q2 ->
+    raw_data_item_size_eq x1;
+    holds_on_raw_data_item_eq (notp Map?) x1;
+    begin match x1, x2 with
+    | Tagged _ v1, Tagged _ v2 ->
+      raw_equiv_list_no_map_no_map (v1 :: q1) (v2 :: q2)
+    | Array _ v1, Array _ v2 ->
+      list_sum_append raw_data_item_size v1 q1;
+      raw_equiv_list_no_map_no_map (v1 `List.Tot.append` q1) (v2 `List.Tot.append` q2);
+      List.Tot.for_all_append (holds_on_raw_data_item (notp Map?)) v1 q1
+    | _ -> raw_equiv_list_no_map_no_map q1 q2
+    end
+  | _ -> ()
+
+let rec raw_equiv_list_no_map_equiv
+  (l1 l2: list raw_data_item)
+: Lemma
+  (requires (raw_equiv_list_no_map l1 l2 == true))
+  (ensures (list_for_all2 raw_equiv l1 l2 == true))
+  (decreases (list_sum raw_data_item_size l1))
+= match l1, l2 with
+  | x1 :: q1, x2 :: q2 ->
+    raw_data_item_size_eq x1;
+    raw_equiv_eq x1 x2;
+    holds_on_raw_data_item_eq (notp Map?) x1;
+    begin match x1, x2 with
+    | Tagged _ v1, Tagged _ v2 ->
+      raw_equiv_list_no_map_equiv (v1 :: q1) (v2 :: q2)
+    | Array _ v1, Array _ v2 ->
+      list_sum_append raw_data_item_size v1 q1;
+      raw_equiv_list_no_map_equiv (v1 `List.Tot.append` q1) (v2 `List.Tot.append` q2);
+      list_for_all2_append raw_equiv v1 q1 v2 q2
+    | _ -> raw_equiv_list_no_map_equiv q1 q2
+    end
+  | _ -> ()
+
+let rec raw_equiv_list_no_map_sym'
+  (l1 l2: list raw_data_item)
+: Lemma
+  (requires (raw_equiv_list_no_map l1 l2 == true))
+  (ensures (raw_equiv_list_no_map l2 l1 == true))
+  (decreases (list_sum raw_data_item_size l1))
+= match l1, l2 with
+  | x1 :: q1, x2 :: q2 ->
+    raw_data_item_size_eq x1;
+    raw_data_item_size_eq x2;
+    begin match x1, x2 with
+    | Array len1 v1, Array len2 v2 ->
+      list_sum_append raw_data_item_size v1 q1;
+      raw_equiv_list_no_map_sym' (v1 `List.Tot.append` q1) (v2 `List.Tot.append` q2)
+    | Tagged tag1 v1, Tagged tag2 v2 ->
+      raw_equiv_list_no_map_sym' (v1 :: q1) (v2 :: q2)
+    | _ -> raw_equiv_list_no_map_sym' q1 q2
+    end
+  | _ -> ()
+
+let raw_equiv_list_no_map_sym
+  (l1 l2: list raw_data_item)
+: Lemma
+  (raw_equiv_list_no_map l1 l2 == raw_equiv_list_no_map l2 l1)
+= Classical.move_requires (raw_equiv_list_no_map_sym' l1) l2;
+  Classical.move_requires (raw_equiv_list_no_map_sym' l2) l1
+
+let rec raw_equiv_equiv_list_no_map
+  (l1 l2: list raw_data_item)
+: Lemma
+  (requires (
+    list_for_all2 raw_equiv l1 l2 == true /\
+    list_for_all2 (prod_or (holds_on_raw_data_item (notp Map?)) (holds_on_raw_data_item (notp Map?))) l1 l2 == true
+  ))
+  (ensures (
+    raw_equiv_list_no_map l1 l2 == true
+  ))
+  (decreases (list_sum raw_data_item_size l1))
+= match l1, l2 with
+  | x1 :: q1, x2 :: q2 ->
+    raw_data_item_size_eq x1;
+    raw_equiv_eq x1 x2;
+    begin match x1, x2 with
+    | Array len1 v1, Array len2 v2 ->
+      list_sum_append raw_data_item_size v1 q1;
+      list_for_all2_append raw_equiv v1 q1 v2 q2;
+      list_for_all2_prod_or_weak (holds_on_raw_data_item (notp Map?)) (holds_on_raw_data_item (notp Map?)) v1 v2;
+      list_for_all2_append (prod_or (holds_on_raw_data_item (notp Map?)) (holds_on_raw_data_item (notp Map?))) v1 q1 v2 q2;
+      raw_equiv_equiv_list_no_map (v1 `List.Tot.append` q1) (v2 `List.Tot.append` q2)
+    | Tagged tag1 v1, Tagged tag2 v2 ->
+      raw_equiv_equiv_list_no_map (v1 :: q1) (v2 :: q2)
+    | _ -> raw_equiv_equiv_list_no_map q1 q2
+    end
+  | _ -> ()
+
+let raw_equiv_list_no_map_eq
+  (l1 l2: list raw_data_item)
+: Lemma
+  (raw_equiv_list_no_map l1 l2 == (list_for_all2 raw_equiv l1 l2 && list_for_all2 (prod_or (holds_on_raw_data_item (notp Map?)) (holds_on_raw_data_item (notp Map?))) l1 l2))
+= if raw_equiv_list_no_map l1 l2
+  then begin
+    raw_equiv_list_no_map_no_map l1 l2;
+    raw_equiv_list_no_map_equiv l1 l2;
+    list_for_all2_length raw_equiv l1 l2;
+    list_for_all2_prod_or_weak (holds_on_raw_data_item (notp Map?)) (holds_on_raw_data_item (notp Map?)) l1 l2
+  end
+  else if (list_for_all2 raw_equiv l1 l2 && list_for_all2 (prod_or (holds_on_raw_data_item (notp Map?)) (holds_on_raw_data_item (notp Map?))) l1 l2)
+  then raw_equiv_equiv_list_no_map l1 l2
+  else ()
+
+let raw_equiv_no_map
+  (x1 x2: raw_data_item)
+: Tot bool
+= raw_equiv_list_no_map [x1] [x2]
+
+let raw_equiv_list_no_map_no_map2
+  (l1 l2: list raw_data_item)
+: Lemma
+  (requires (raw_equiv_list_no_map l1 l2 == true))
+  (ensures (List.Tot.for_all (holds_on_raw_data_item (notp Map?)) l1 == true /\
+    List.Tot.for_all (holds_on_raw_data_item (notp Map?)) l2 == true
+  ))
+= raw_equiv_list_no_map_no_map l1 l2;
+  raw_equiv_list_no_map_sym l1 l2;
+  raw_equiv_list_no_map_no_map l2 l1
+
+let rec raw_equiv_list_no_map_eq'
+  (l1 l2: list raw_data_item)
+: Lemma
+  (ensures (raw_equiv_list_no_map l1 l2 == list_for_all2 raw_equiv_no_map l1 l2))
+  (decreases l1)
+= raw_equiv_list_no_map_eq l1 l2;
+  match l1, l2 with
+  | a1 :: q1, a2 :: q2 ->
+    raw_equiv_list_no_map_eq [a1] [a2];
+    raw_equiv_list_no_map_eq q1 q2;
+    raw_equiv_list_no_map_eq' q1 q2
+  | _ -> ()
+
+let no_maps_in_keys_elem
   (x: raw_data_item)
 : Tot bool
 = match x with
-  | Map _ v ->
-    no_map_and_no_repeats_keys_map v
+  | Map _ v -> List.Tot.for_all (holds_on_raw_data_item (notp Map?)) (List.Tot.map fst v)
   | _ -> true
 
-let no_map_and_no_repeats_keys
-: (x: raw_data_item) -> Tot bool
-= holds_on_raw_data_item no_map_and_no_repeats_keys_elem
-
-let list_no_repeats_no_setoid_repeats
-  (#key: Type)
-  (#value: Type)
-  (equiv: key -> key -> bool)
-  (l: list (key & value))
-  (prf: (x: (key & value)) -> (y: (key & value)) -> Lemma
-    (requires (List.Tot.memP x l /\
-      List.Tot.memP y l /\
-      fst x `equiv` fst y
-    ))
-    (ensures (x == y))
-  )
-: Lemma
-  (requires (List.Tot.no_repeats_p (List.Tot.map fst l)))
-  (ensures (list_no_setoid_repeats (map_entry_order equiv _) l))
-= admit ()
-
-let no_map_and_no_repeats_keys_map_list_no_setoid_repeats
-  (v: list (raw_data_item & raw_data_item))
-: Lemma
-  (requires (
-    no_map_and_no_repeats_keys_map v == true /\
-    List.Tot.for_all (holds_on_pair no_map_and_no_repeats_keys) v == true
-  ))
-  (ensures (
-    list_no_setoid_repeats (map_entry_order raw_equiv _) v
-  ))
-= admit ()
-
-let no_map_and_no_repeats_keys_valid
-  (x: raw_data_item)
-: Lemma
-  (requires (no_map_and_no_repeats_keys x == true))
-  (ensures (valid_raw_data_item x == true))
-= holds_on_raw_data_item_implies
-    no_map_and_no_repeats_keys_elem
-    valid_raw_data_item_elem
-    (fun x ->
-      if no_map_and_no_repeats_keys x
-      then begin
-        holds_on_raw_data_item_eq no_map_and_no_repeats_keys_elem x;
-        match x with
-        | Map len v ->
-          assert_norm (no_map_and_no_repeats_keys == holds_on_raw_data_item no_map_and_no_repeats_keys_elem);
-          no_map_and_no_repeats_keys_map_list_no_setoid_repeats v
-        | _ -> ()
-      end
-    )
-    x
+let no_maps_in_keys = holds_on_raw_data_item no_maps_in_keys_elem
